first step at journalistimpl

Impl/JournalistImpl.i.dfy
@@ -19,34 +19,12 @@ module JournalistImpl {
 
   import JournalistModel
 
-  class Journalist {
-    var journalEntries: array<JournalEntry>;
-    var start: uint64;
-    var len1: uint64;
-    var len2: uint64;
-
-    var replayJournal: seq<JournalEntry>;
-    var replayIdx: uint64;
-
-    var journalFront: Option<seq<JournalBlock>>;
-    var journalBack: Option<seq<JournalBlock>>;
-    
-    var writtenJournalBlocks: uint64;
-    var frozenJournalBlocks: uint64;
-    var inMemoryWeight: uint64;
-
-    ghost var Repr: set<object>;
-
-    protected predicate ReprInv()
-    reads this
-    ensures ReprInv() ==> this in Repr
-    {
-      Repr == {this, this.journalEntries}
-    }
-
-    protected function I() : JournalistModel.JournalistModel
-    reads this, this.Repr
-    requires ReprInv()
+  linear datatype Journalist = Journalist(journalEntries: seq<JournalEntry>, start: uint64,
+    len1: uint64, len2: uint64, replayJournal: seq<JournalEntry>, replayIdx: uint64, 
+    journalFront: Option<seq<JournalBlock>>, journalBack: Option<seq<JournalBlock>>, writtenJournalBlocks: uint64,
+    frozenJournalBlocks: uint64, inMemoryWeight: uint64)
+  {
+    function I() : JournalistModel.JournalistModel
     {
       JournalistModel.JournalistModel(
         this.journalEntries[..],
@@ -63,46 +41,28 @@ module JournalistImpl {
     }
 
     predicate WF()
-    reads this, this.Repr
     {
-      && ReprInv()
       && JournalistModel.WF(I())
     }
 
-    protected predicate Inv()
-    reads this, this.Repr
-    ensures Inv() ==> ReprInv()
+    predicate Inv()
     {
-      && ReprInv()
       && JournalistModel.Inv(I())
     }
 
-    constructor()
-    ensures Inv()
-    ensures fresh(Repr)
-    ensures I() == JournalistModel.JournalistConstructor()
+    static method NewJournal() returns (linear j: Journalist)
+    ensures j.Inv()
+    ensures j.I() == JournalistModel.JournalistConstructor()
     {
-      new;
-      this.journalEntries := NativeArrays.newArrayFill(
-          4096,
-          JournalInsert([], []));
-      this.start := 0;
-      this.len1 := 0;
-      this.len2 := 0;
-      this.replayJournal := [];
-      this.replayIdx := 0;
-      this.journalFront := None;
-      this.journalBack := None;
-      this.writtenJournalBlocks := 0;
-      this.frozenJournalBlocks := 0;
-      this.inMemoryWeight := 0;
+      j := Journalist(
+        [JournalInsert([], [])], 0, 0, 0,
+        [], 0, None, None, 0, 0, 0);
 
-      Repr := {this, this.journalEntries};
       JournalistModel.reveal_JournalistConstructor();
-      assert I() == JournalistModel.JournalistConstructor();
+      assert j.I() == JournalistModel.JournalistConstructor();
     }
 
-    method hasFrozenJournal() returns (b: bool)
+    shared method hasFrozenJournal() returns (b: bool)
     requires Inv()
     ensures b == JournalistModel.hasFrozenJournal(I())
     {
@@ -110,7 +70,7 @@ module JournalistImpl {
       return this.len1 != 0;
     }
 
-    method hasInMemoryJournal() returns (b: bool)
+    shared method hasInMemoryJournal() returns (b: bool)
     requires Inv()
     ensures b == JournalistModel.hasInMemoryJournal(I())
     {
@@ -118,280 +78,281 @@ module JournalistImpl {
       return this.len2 != 0;
     }
 
-    method packageFrozenJournal() returns (s: seq<byte>)
-    requires Inv()
-    requires JournalistModel.packageFrozenJournal.requires(I())
-    modifies this.Repr
-    ensures Repr == old(Repr)
-    ensures Inv()
-    ensures (I(), s) == JournalistModel.packageFrozenJournal(old(I()))
-    {
-      JournalistModel.reveal_packageFrozenJournal();
-      reveal_WeightJournalEntries();
-      JournalistModel.reveal_I(I());
+    // method packageFrozenJournal() returns (s: seq<byte>)
+    // requires Inv()
+    // requires JournalistModel.packageFrozenJournal.requires(I())
+    // modifies this.Repr
+    // ensures Repr == old(Repr)
+    // ensures Inv()
+    // ensures (I(), s) == JournalistModel.packageFrozenJournal(old(I()))
+    // {
+    //   JournalistModel.reveal_packageFrozenJournal();
+    //   reveal_WeightJournalEntries();
+    //   JournalistModel.reveal_I(I());
 
-      s := MarshallJournalEntries(
-        this.journalEntries,
-        this.start,
-        this.len1,
-        this.frozenJournalBlocks);
+    //   s := MarshallJournalEntries(
+    //     this.journalEntries,
+    //     this.start,
+    //     this.len1,
+    //     this.frozenJournalBlocks);
 
-      this.start := JournalistModel.basic_mod(this.start + this.len1,
-          this.journalEntries.Length as uint64);
-      this.len1 := 0;
-      this.writtenJournalBlocks :=
-          this.writtenJournalBlocks + this.frozenJournalBlocks;
-      this.frozenJournalBlocks := 0;
-    }
+    //   this.start := JournalistModel.basic_mod(this.start + this.len1,
+    //       this.journalEntries.Length as uint64);
+    //   this.len1 := 0;
+    //   this.writtenJournalBlocks :=
+    //       this.writtenJournalBlocks + this.frozenJournalBlocks;
+    //   this.frozenJournalBlocks := 0;
+    // }
 
-    method packageInMemoryJournal() returns (s: seq<byte>)
-    requires Inv()
-    requires JournalistModel.packageInMemoryJournal.requires(I())
-    modifies this.Repr
-    ensures Repr == old(Repr)
-    ensures Inv()
-    ensures (I(), s) == JournalistModel.packageInMemoryJournal(old(I()))
-    {
-      JournalistModel.reveal_packageInMemoryJournal();
-      reveal_WeightJournalEntries();
-      JournalistModel.reveal_I(I());
+    // method packageInMemoryJournal() returns (s: seq<byte>)
+    // requires Inv()
+    // requires JournalistModel.packageInMemoryJournal.requires(I())
+    // modifies this.Repr
+    // ensures Repr == old(Repr)
+    // ensures Inv()
+    // ensures (I(), s) == JournalistModel.packageInMemoryJournal(old(I()))
+    // {
+    //   JournalistModel.reveal_packageInMemoryJournal();
+    //   reveal_WeightJournalEntries();
+    //   JournalistModel.reveal_I(I());
 
-      var numBlocks := (this.inMemoryWeight + 4064 - 1) / 4064;
-      s := MarshallJournalEntries(
-        this.journalEntries,
-        this.start,
-        this.len2,
-        numBlocks);
+    //   var numBlocks := (this.inMemoryWeight + 4064 - 1) / 4064;
+    //   s := MarshallJournalEntries(
+    //     this.journalEntries,
+    //     this.start,
+    //     this.len2,
+    //     numBlocks);
 
-      this.start := 0;
-      this.len2 := 0;
-      this.inMemoryWeight := 0;
-      this.writtenJournalBlocks := this.writtenJournalBlocks + numBlocks;
-    }
+    //   this.start := 0;
+    //   this.len2 := 0;
+    //   this.inMemoryWeight := 0;
+    //   this.writtenJournalBlocks := this.writtenJournalBlocks + numBlocks;
+    // }
 
-    method getWrittenJournalLen()
-    returns (len : uint64)
-    requires Inv()
-    ensures len == JournalistModel.getWrittenJournalLen(I())
-    {
-      return this.writtenJournalBlocks;
-    }
+    // method getWrittenJournalLen()
+    // returns (len : uint64)
+    // requires Inv()
+    // ensures len == JournalistModel.getWrittenJournalLen(I())
+    // {
+    //   return this.writtenJournalBlocks;
+    // }
 
-    method setWrittenJournalLen(len: uint64)
-    requires Inv()
-    requires JournalistModel.setWrittenJournalLen.requires(I(), len)
-    modifies Repr
-    ensures Repr == old(Repr)
-    ensures Inv()
-    ensures I() == JournalistModel.setWrittenJournalLen(old(I()), len)
-    {
-      this.writtenJournalBlocks := len;
-      this.frozenJournalBlocks := 0;
-      assert I() == JournalistModel.setWrittenJournalLen(old(I()), len);
-    }
+  //   linear inout method setWrittenJournalLen(len: uint64):
+  //   requires Inv()
+  //   requires JournalistModel.setWrittenJournalLen.requires(I(), len)
+  //   ensures Inv()
+  //   ensures I() == JournalistModel.setWrittenJournalLen(old(I()), len)
+  //   {
+  //     // this = self 
+  //     // old(this) = old_self
 
-    method updateWrittenJournalLen(len: uint64)
-    requires Inv()
-    requires JournalistModel.updateWrittenJournalLen.requires(I(), len)
-    modifies Repr
-    ensures Repr == old(Repr)
-    ensures Inv()
-    ensures I() == JournalistModel.updateWrittenJournalLen(old(I()), len)
-    {
-      this.writtenJournalBlocks := len;
-      assert I() ==
-        JournalistModel.updateWrittenJournalLen(old(I()), len);
-    }
+  //     inout self.writtenJournalBlocks := len;
+  //     inout self.frozenJournalBlocks := 0;
+  //     assert I() == JournalistModel.setWrittenJournalLen(old_self.I(), len);
+  //   }
 
-    method freeze()
-    requires Inv()
-    modifies Repr
-    ensures Repr == old(Repr)
-    ensures Inv()
-    ensures I() == JournalistModel.freeze(old(I()))
-    {
-      JournalistModel.reveal_freeze();
+  //   method updateWrittenJournalLen(len: uint64)
+  //   requires Inv()
+  //   requires JournalistModel.updateWrittenJournalLen.requires(I(), len)
+  //   modifies Repr
+  //   ensures Repr == old(Repr)
+  //   ensures Inv()
+  //   ensures I() == JournalistModel.updateWrittenJournalLen(old(I()), len)
+  //   {
+  //     this.writtenJournalBlocks := len;
+  //     assert I() ==
+  //       JournalistModel.updateWrittenJournalLen(old(I()), len);
+  //   }
 
-      this.len1 := this.len1 + this.len2;
-      this.len2 := 0;
-      this.frozenJournalBlocks := this.frozenJournalBlocks
-          + (this.inMemoryWeight + 4064 - 1) / 4064;
-      this.inMemoryWeight := 0;
+  //   method freeze()
+  //   requires Inv()
+  //   modifies Repr
+  //   ensures Repr == old(Repr)
+  //   ensures Inv()
+  //   ensures I() == JournalistModel.freeze(old(I()))
+  //   {
+  //     JournalistModel.reveal_freeze();
 
-      assert I() == JournalistModel.freeze(old(I()));
-    }
+  //     this.len1 := this.len1 + this.len2;
+  //     this.len2 := 0;
+  //     this.frozenJournalBlocks := this.frozenJournalBlocks
+  //         + (this.inMemoryWeight + 4064 - 1) / 4064;
+  //     this.inMemoryWeight := 0;
 
-    method canAppend(je: JournalEntry)
-    returns (b: bool)
-    requires Inv()
-    ensures b == JournalistModel.canAppend(I(), je)
-    {
-      JournalistModel.reveal_canAppend();
+  //     assert I() == JournalistModel.freeze(old(I()));
+  //   }
 
-      b := 4064 * (writtenJournalBlocks + frozenJournalBlocks)
-          + inMemoryWeight
-          + WeightJournalEntryUint64(je)
-          + (if len2 == 0 then 8 else 0)
-        <= 4064 * NumJournalBlocks();
-    }
+  //   method canAppend(je: JournalEntry)
+  //   returns (b: bool)
+  //   requires Inv()
+  //   ensures b == JournalistModel.canAppend(I(), je)
+  //   {
+  //     JournalistModel.reveal_canAppend();
 
-    method append(je: JournalEntry)
-    requires Inv()
-    requires JournalistModel.canAppend(I(), je)
-    modifies Repr
-    ensures forall o | o in Repr :: o in old(Repr) || fresh(o)
-    ensures Inv()
-    ensures I() == JournalistModel.append(old(I()), je)
-    {
-      JournalistModel.reveal_append();
+  //     b := 4064 * (writtenJournalBlocks + frozenJournalBlocks)
+  //         + inMemoryWeight
+  //         + WeightJournalEntryUint64(je)
+  //         + (if len2 == 0 then 8 else 0)
+  //       <= 4064 * NumJournalBlocks();
+  //   }
 
-      if this.len1 + this.len2 < this.journalEntries.Length as uint64 {
-        var idx := JournalistModel.basic_mod(
-            start + len1 + len2,
-            this.journalEntries.Length as uint64);
-        this.journalEntries[idx] := je;
-      } else {
-        var newLen: uint64 := this.journalEntries.Length as uint64 * 2;
-        var newArray := NativeArrays.newArrayFill(
-            newLen,
-            JournalInsert([], []));
-        NativeArrays.CopyArrayIntoDifferentArray(
-            this.journalEntries,
-            this.start,
-            newArray,
-            0,
-            this.journalEntries.Length as uint64 - this.start);
-        NativeArrays.CopyArrayIntoDifferentArray(
-            this.journalEntries,
-            0,
-            newArray,
-            this.journalEntries.Length as uint64 - this.start,
-            this.start);
-        newArray[this.journalEntries.Length as uint64] := je;
+  //   method append(je: JournalEntry)
+  //   requires Inv()
+  //   requires JournalistModel.canAppend(I(), je)
+  //   modifies Repr
+  //   ensures forall o | o in Repr :: o in old(Repr) || fresh(o)
+  //   ensures Inv()
+  //   ensures I() == JournalistModel.append(old(I()), je)
+  //   {
+  //     JournalistModel.reveal_append();
 
-        calc {
-          newArray[..];
-          journalEntries[start..]
-            + journalEntries[..start]
-            + [je]
-            + fill((newLen as int - journalEntries.Length - 1) as int, JournalInsert([], []));
-        }
+  //     if this.len1 + this.len2 < this.journalEntries.Length as uint64 {
+  //       var idx := JournalistModel.basic_mod(
+  //           start + len1 + len2,
+  //           this.journalEntries.Length as uint64);
+  //       this.journalEntries[idx] := je;
+  //     } else {
+  //       var newLen: uint64 := this.journalEntries.Length as uint64 * 2;
+  //       var newArray := NativeArrays.newArrayFill(
+  //           newLen,
+  //           JournalInsert([], []));
+  //       NativeArrays.CopyArrayIntoDifferentArray(
+  //           this.journalEntries,
+  //           this.start,
+  //           newArray,
+  //           0,
+  //           this.journalEntries.Length as uint64 - this.start);
+  //       NativeArrays.CopyArrayIntoDifferentArray(
+  //           this.journalEntries,
+  //           0,
+  //           newArray,
+  //           this.journalEntries.Length as uint64 - this.start,
+  //           this.start);
+  //       newArray[this.journalEntries.Length as uint64] := je;
 
-        this.journalEntries := newArray;
-        this.start := 0;
-      }
+  //       calc {
+  //         newArray[..];
+  //         journalEntries[start..]
+  //           + journalEntries[..start]
+  //           + [je]
+  //           + fill((newLen as int - journalEntries.Length - 1) as int, JournalInsert([], []));
+  //       }
 
-      this.inMemoryWeight := this.inMemoryWeight
-          + WeightJournalEntryUint64(je)
-          + (if this.len2 == 0 then 8 else 0);
-      this.len2 := this.len2 + 1;
+  //       this.journalEntries := newArray;
+  //       this.start := 0;
+  //     }
 
-      Repr := {this, this.journalEntries};
-      //assert I().journalEntries == JournalistModel.append(old(I()), je).journalEntries;
-      //assert I().start == JournalistModel.append(old(I()), je).start;
-      assert I() == JournalistModel.append(old(I()), je);
-    }
+  //     this.inMemoryWeight := this.inMemoryWeight
+  //         + WeightJournalEntryUint64(je)
+  //         + (if this.len2 == 0 then 8 else 0);
+  //     this.len2 := this.len2 + 1;
 
-    method isReplayEmpty()
-    returns (b: bool)
-    requires Inv()
-    ensures b == JournalistModel.isReplayEmpty(I())
-    {
-      JournalistModel.reveal_isReplayEmpty();
-      b := (replayIdx == |replayJournal| as uint64);
-    }
+  //     Repr := {this, this.journalEntries};
+  //     //assert I().journalEntries == JournalistModel.append(old(I()), je).journalEntries;
+  //     //assert I().start == JournalistModel.append(old(I()), je).start;
+  //     assert I() == JournalistModel.append(old(I()), je);
+  //   }
 
-    method replayJournalTop()
-    returns (je: JournalEntry)
-    requires Inv()
-    requires JournalistModel.I(I()).replayJournal != []
-    ensures je == JournalistModel.replayJournalTop(I())
-    {
-      JournalistModel.reveal_replayJournalTop();
-      JournalistModel.reveal_I(I());
-      je := replayJournal[replayIdx];
-    }
+  //   method isReplayEmpty()
+  //   returns (b: bool)
+  //   requires Inv()
+  //   ensures b == JournalistModel.isReplayEmpty(I())
+  //   {
+  //     JournalistModel.reveal_isReplayEmpty();
+  //     b := (replayIdx == |replayJournal| as uint64);
+  //   }
 
-    method replayJournalPop()
-    requires Inv()
-    requires JournalistModel.I(I()).replayJournal != []
-    modifies Repr
-    ensures Inv()
-    ensures Repr == old(Repr)
-    ensures I() == JournalistModel.replayJournalPop(old(I()))
-    {
-      JournalistModel.reveal_replayJournalPop();
-      JournalistModel.reveal_I(I());
-      replayIdx := replayIdx + 1;
-    }
+  //   method replayJournalTop()
+  //   returns (je: JournalEntry)
+  //   requires Inv()
+  //   requires JournalistModel.I(I()).replayJournal != []
+  //   ensures je == JournalistModel.replayJournalTop(I())
+  //   {
+  //     JournalistModel.reveal_replayJournalTop();
+  //     JournalistModel.reveal_I(I());
+  //     je := replayJournal[replayIdx];
+  //   }
 
-    method setFront(jr: JournalRange)
-    requires Inv()
-    requires forall i | 0 <= i < |jr| :: |jr[i]| == 4064
-    requires |jr| <= NumJournalBlocks() as int
-    modifies Repr
-    ensures Inv()
-    ensures Repr == old(Repr)
-    ensures I() == JournalistModel.setFront(old(I()), jr)
-    {
-      JournalistModel.reveal_setFront();
-      journalFront := Some(jr);
-    }
+  //   method replayJournalPop()
+  //   requires Inv()
+  //   requires JournalistModel.I(I()).replayJournal != []
+  //   modifies Repr
+  //   ensures Inv()
+  //   ensures Repr == old(Repr)
+  //   ensures I() == JournalistModel.replayJournalPop(old(I()))
+  //   {
+  //     JournalistModel.reveal_replayJournalPop();
+  //     JournalistModel.reveal_I(I());
+  //     replayIdx := replayIdx + 1;
+  //   }
 
-    method setBack(jr: JournalRange)
-    requires Inv()
-    requires forall i | 0 <= i < |jr| :: |jr[i]| == 4064
-    requires |jr| <= NumJournalBlocks() as int
-    modifies Repr
-    ensures Inv()
-    ensures Repr == old(Repr)
-    ensures I() == JournalistModel.setBack(old(I()), jr)
-    {
-      JournalistModel.reveal_setBack();
-      journalBack := Some(jr);
-    }
+  //   method setFront(jr: JournalRange)
+  //   requires Inv()
+  //   requires forall i | 0 <= i < |jr| :: |jr[i]| == 4064
+  //   requires |jr| <= NumJournalBlocks() as int
+  //   modifies Repr
+  //   ensures Inv()
+  //   ensures Repr == old(Repr)
+  //   ensures I() == JournalistModel.setFront(old(I()), jr)
+  //   {
+  //     JournalistModel.reveal_setFront();
+  //     journalFront := Some(jr);
+  //   }
 
-    method parseJournals()
-    returns (success: bool)
-    requires Inv()
-    modifies Repr
-    ensures Inv()
-    ensures Repr == old(Repr)
-    ensures (I(), success) == JournalistModel.parseJournals(old(I()))
-    {
-      JournalistModel.reveal_parseJournals();
-      JournalistModel.reveal_I(I());
-      var fullRange :=
-        (if journalFront.Some? then journalFront.value else []) +
-        (if journalBack.Some? then journalBack.value else []);
-      var p := JournalistParsingImpl.ParseJournalRange(fullRange);
-      if p.Some? && |p.value| as uint64 <= JournalistModel.MaxPossibleEntries() {
-        journalFront := None;
-        journalBack := None;
-        replayJournal := p.value;
-        replayIdx := 0;
-        return true;
-      } else {
-        return false;
-      }
-    }
+  //   method setBack(jr: JournalRange)
+  //   requires Inv()
+  //   requires forall i | 0 <= i < |jr| :: |jr[i]| == 4064
+  //   requires |jr| <= NumJournalBlocks() as int
+  //   modifies Repr
+  //   ensures Inv()
+  //   ensures Repr == old(Repr)
+  //   ensures I() == JournalistModel.setBack(old(I()), jr)
+  //   {
+  //     JournalistModel.reveal_setBack();
+  //     journalBack := Some(jr);
+  //   }
 
-    method hasFront()
-    returns (b: bool)
-    requires Inv()
-    ensures b == JournalistModel.hasFront(I())
-    {
-      JournalistModel.reveal_hasFront();
-      b := journalFront.Some?;
-    }
+  //   method parseJournals()
+  //   returns (success: bool)
+  //   requires Inv()
+  //   modifies Repr
+  //   ensures Inv()
+  //   ensures Repr == old(Repr)
+  //   ensures (I(), success) == JournalistModel.parseJournals(old(I()))
+  //   {
+  //     JournalistModel.reveal_parseJournals();
+  //     JournalistModel.reveal_I(I());
+  //     var fullRange :=
+  //       (if journalFront.Some? then journalFront.value else []) +
+  //       (if journalBack.Some? then journalBack.value else []);
+  //     var p := JournalistParsingImpl.ParseJournalRange(fullRange);
+  //     if p.Some? && |p.value| as uint64 <= JournalistModel.MaxPossibleEntries() {
+  //       journalFront := None;
+  //       journalBack := None;
+  //       replayJournal := p.value;
+  //       replayIdx := 0;
+  //       return true;
+  //     } else {
+  //       return false;
+  //     }
+  //   }
 
-    method hasBack()
-    returns (b: bool)
-    requires Inv()
-    ensures b == JournalistModel.hasBack(I())
-    {
-      JournalistModel.reveal_hasBack();
-      b := journalBack.Some?;
-    }
+  //   method hasFront()
+  //   returns (b: bool)
+  //   requires Inv()
+  //   ensures b == JournalistModel.hasFront(I())
+  //   {
+  //     JournalistModel.reveal_hasFront();
+  //     b := journalFront.Some?;
+  //   }
+
+  //   method hasBack()
+  //   returns (b: bool)
+  //   requires Inv()
+  //   ensures b == JournalistModel.hasBack(I())
+  //   {
+  //     JournalistModel.reveal_hasBack();
+  //     b := journalBack.Some?;
+  //   }
   }
 }
