j
@@ -1,0 +1,145 @@
+diff --git a/Impl/JournalistImpl.i.dfy b/Impl/JournalistImpl.i.dfy
+index 67f652ba..37c62d65 100644
+--- a/Impl/JournalistImpl.i.dfy
++++ b/Impl/JournalistImpl.i.dfy
+@@ -19,34 +19,12 @@ module JournalistImpl {
+ 
+   import JournalistModel
+ 
+-  class Journalist {
+-    var journalEntries: array<JournalEntry>;
+-    var start: uint64;
+-    var len1: uint64;
+-    var len2: uint64;
+-
+-    var replayJournal: seq<JournalEntry>;
+-    var replayIdx: uint64;
+-
+-    var journalFront: Option<seq<JournalBlock>>;
+-    var journalBack: Option<seq<JournalBlock>>;
+-    
+-    var writtenJournalBlocks: uint64;
+-    var frozenJournalBlocks: uint64;
+-    var inMemoryWeight: uint64;
+-
+-    ghost var Repr: set<object>;
+-
+-    protected predicate ReprInv()
+-    reads this
+-    ensures ReprInv() ==> this in Repr
+-    {
+-      Repr == {this, this.journalEntries}
+-    }
+-
+-    protected function I() : JournalistModel.JournalistModel
+-    reads this, this.Repr
+-    requires ReprInv()
++  linear datatype Journalist = Journalist(journalEntries: seq<JournalEntry>, start: uint64,
++    len1: uint64, len2: uint64, replayJournal: seq<JournalEntry>, replayIdx: uint64, 
++    journalFront: Option<seq<JournalBlock>>, journalBack: Option<seq<JournalBlock>>, writtenJournalBlocks: uint64,
++    frozenJournalBlocks: uint64, inMemoryWeight: uint64)
++  {
++    function I() : JournalistModel.JournalistModel
+     {
+       JournalistModel.JournalistModel(
+         this.journalEntries[..],
+@@ -63,46 +41,38 @@ module JournalistImpl {
+     }
+ 
+     predicate WF()
+-    reads this, this.Repr
+     {
+-      && ReprInv()
+       && JournalistModel.WF(I())
+     }
+ 
+-    protected predicate Inv()
+-    reads this, this.Repr
+-    ensures Inv() ==> ReprInv()
++    predicate Inv()
+     {
+-      && ReprInv()
+       && JournalistModel.Inv(I())
+     }
+ 
+-    constructor()
+-    ensures Inv()
+-    ensures fresh(Repr)
+-    ensures I() == JournalistModel.JournalistConstructor()
++    static method NewJournal(): (linear j: Journalist)
++    ensures j.Inv()
++    ensures j.I() == JournalistModel.JournalistConstructor()
+     {
+-      new;
+-      this.journalEntries := NativeArrays.newArrayFill(
+-          4096,
+-          JournalInsert([], []));
+-      this.start := 0;
+-      this.len1 := 0;
+-      this.len2 := 0;
+-      this.replayJournal := [];
+-      this.replayIdx := 0;
+-      this.journalFront := None;
+-      this.journalBack := None;
+-      this.writtenJournalBlocks := 0;
+-      this.frozenJournalBlocks := 0;
+-      this.inMemoryWeight := 0;
++      linear var j := Journalist;
++      j.journalEntries := JournalInsert([], []);
++      j.start := 0;
++      j.len1 := 0;
++      j.len2 := 0;
++      j.replayJournal := [];
++      j.replayIdx := 0;
++      j.journalFront := None;
++      j.journalBack := None;
++      j.writtenJournalBlocks := 0;
++      j.frozenJournalBlocks := 0;
++      j.inMemoryWeight := 0;
+ 
+-      Repr := {this, this.journalEntries};
+       JournalistModel.reveal_JournalistConstructor();
+-      assert I() == JournalistModel.JournalistConstructor();
++      assert j.I() == JournalistModel.JournalistConstructor();
++      return j;
+     }
+ 
+-    method hasFrozenJournal() returns (b: bool)
++    shared method hasFrozenJournal() returns (b: bool)
+     requires Inv()
+     ensures b == JournalistModel.hasFrozenJournal(I())
+     {
+@@ -110,7 +80,7 @@ module JournalistImpl {
+       return this.len1 != 0;
+     }
+ 
+-    method hasInMemoryJournal() returns (b: bool)
++    shared method hasInMemoryJournal() returns (b: bool)
+     requires Inv()
+     ensures b == JournalistModel.hasInMemoryJournal(I())
+     {
+@@ -177,17 +147,18 @@ module JournalistImpl {
+       return this.writtenJournalBlocks;
+     }
+ 
+-    method setWrittenJournalLen(len: uint64)
++    linear inout method setWrittenJournalLen(len: uint64):
+     requires Inv()
+     requires JournalistModel.setWrittenJournalLen.requires(I(), len)
+-    modifies Repr
+-    ensures Repr == old(Repr)
+     ensures Inv()
+     ensures I() == JournalistModel.setWrittenJournalLen(old(I()), len)
+     {
+-      this.writtenJournalBlocks := len;
+-      this.frozenJournalBlocks := 0;
+-      assert I() == JournalistModel.setWrittenJournalLen(old(I()), len);
++      // this = self 
++      // old(this) = old_self
++
++      inout self.writtenJournalBlocks := len;
++      inout self.frozenJournalBlocks := 0;
++      assert I() == JournalistModel.setWrittenJournalLen(old_self.I(), len);
+     }
+ 
+     method updateWrittenJournalLen(len: uint64)
